\documentclass[addpoints]{exam}
\makeatletter
\expandafter\providecommand\expandafter*\csname ver@framed.sty\endcsname
{2003/07/21 v0.8a Simulated by exam}
\makeatother
\usepackage{framed}

%\printanswers

\usepackage{amsmath,bigstrut,minted,url,graphicx,tikz,marvosym,rotating}
\usepackage{ebproof}

\pagestyle{headandfoot}
\runningheadrule
\firstpageheader{}{}{Page \thepage\ of \numpages}
\runningheader{CS 321}{Sample Problems}{Page \thepage\ of \numpages}
\firstpagefooter{}{}{}
\runningfooter{}{}{}
              
\newcommand{\EJDG}[3]{#1 \vdash #2 \Rightarrow #3}
\newcommand{\TJDG}[3]{#1 \vdash #2 : #3}
\renewcommand{\L}[2]{\lambda #1.#2}

\begin{document}

\begin{center}
{\Large \textbf{
    Ozyegin University\\
    CS 321 Programming Languages\\
    Sample Problems on Lambda Calculus
}}
\end{center}

\begin{questions}
  \question
  Apply \textbf{one} step of beta reduction on the following lambda terms,
  if possible. If there is no beta reduction possibility, write NORMAL FORM.

  \begin{itemize}
  \item $(\lambda x\,.\,x\,y\,z)\,a\,b\,c~\Rightarrow~$\fillin[ $(a\,y\,z)\,b\,c$ ][4cm]\\[1em]
  \item $(\lambda w\,.\,\lambda p\,.\,p\,w)~\Rightarrow~$\fillin[ NORMAL FORM ][4cm]\\[1em]
  \item $(\lambda x\,.\,\lambda y\,.\,x\,(y\,x))\,(\lambda w\,.\,\lambda v\,.\,w)\,(\lambda z\,.\,z)~\Rightarrow~$\fillin[ $(\lambda y\,.\,(\lambda w\,.\,\lambda v\,.\,w)\,(y\,(\lambda w\,.\,\lambda v\,.\,w)))\,(\lambda z\,.\,z)$ ][8cm]\\[1em]
  \item $(\lambda z\,.\,z\,(\lambda k\,.\,k)\,m)~\Rightarrow~$\fillin[ NORMAL FORM ][4cm]\\[1em]
  \item $(\lambda u\,.\,(\lambda x\,.\,x\,u)\,(\lambda y\,.\,u))~\Rightarrow~$\fillin[ $(\lambda u\,.\,(\lambda y\,.\,u)\,u)$ ][4cm]\\[1em]
  \item $(\lambda n\,.\,n\,n)\,(\lambda n\,.\,n\,n)~\Rightarrow~$\fillin[ $(\lambda n\,.\,n\,n)\,(\lambda n\,.\,n\,n)$ ][4cm]\\[1em]
  \item $(\lambda g\,.\,(\lambda h\,.\,h)\,g)~\Rightarrow~$\fillin[ $(\lambda g\,.\,g)$ ][4cm]\\[1em]
  \end{itemize}
  \begin{solution}
    See \url{https://vimeo.com/250076161}
  \end{solution}
  

  \question
  Reduce the following lambda term to its normal form. If a normal form
  does not exist, show that the term does not converge.

  \[
  (\lambda x.\;\lambda y.\;x~(y~x))~(\lambda w.\;\lambda v.\;w)~(\lambda z.\;z)
  \]
  \begin{solutionbox}{5cm}
    See \url{https://vimeo.com/250078355}
    \begin{align*}
      & (\lambda x.\;\lambda y.\;x~(y~x))~(\lambda w.\;\lambda v.\;w)~(\lambda z.\;z)\\
      & \Rightarrow (\lambda y.\;(\lambda w.\;\lambda v.\;w)~(y~(\lambda w.\;\lambda v.\;w)))~(\lambda z.\;z)\\
      & \Rightarrow (\lambda w.\;\lambda v.\;w)~((\lambda z.\;z)~(\lambda w.\;\lambda v.\;w))\\
      & \Rightarrow (\lambda w.\;\lambda v.\;w)~(\lambda w.\;\lambda v.\;w)\\
      & \Rightarrow (\lambda v.\;(\lambda w.\;\lambda v.\;w))\\
    \end{align*}
  \end{solutionbox}

  \newpage
  \question
  Reduce the following lambda expression to its normal form.

  \[
    (\L{f}{\L{m}{\L{p}{m\,(f\,m\,p)}}})\;(\L{y}{\L{z}{y\,z}})\;(\L{w}{w})
  \]

  \begin{solutionbox}{5cm}
    See \url{https://vimeo.com/250079704}
    \begin{align*}
      & (\L{f}{\L{m}{\L{p}{m\,(f\,m\,p)}}})\;(\L{y}{\L{z}{y\,z}})\;(\L{w}{w})\\
      & \Rightarrow (\L{m}{\L{p}{m\,((\L{y}{\L{z}{y\,z}})\,m\,p)}})\;(\L{w}{w})\\
      & \Rightarrow \L{p}{(\L{w}{w})\,((\L{y}{\L{z}{y\,z}})\,(\L{w}{w})\,p)}\\
      & \Rightarrow \L{p}{((\L{y}{\L{z}{y\,z}})\,(\L{w}{w})\,p)}\\
      & \Rightarrow \L{p}{((\L{z}{(\L{w}{w})\,z})\,p)}\\
      & \Rightarrow \L{p}{((\L{w}{w})\,p)}\\
      & \Rightarrow \L{p}{p}\\
    \end{align*}
  \end{solutionbox}


  \question
  The following are the Church encodings for boolean values and conditional expression.
  Write down an encoding for logical \emph{and}.

  \begin{align*}
    \textbf{true} & = \lambda a. \lambda b.~a \\
    \textbf{false}& = \lambda a. \lambda b.~b \\
    \textbf{if}   & = \lambda c. \lambda t. \lambda e.~c~t~e\\
    \textbf{and}  & = \textrm{\fillin[ $\lambda p. \lambda q.~p~q~\textbf{false}$ ][3.5cm] }\\
  \end{align*}
  \begin{solution}
    See \url{https://vimeo.com/250079905}
  \end{solution}

  \newpage
  \question
  Using the encodings below, show that \textbf{mult 3 2} is \textbf{6}.
  \begin{align*}
    \textbf{0} & = (\L{f}{\L{x}{x}})\\
    \textbf{1} & = (\L{f}{\L{x}{f x}})\\
    \textbf{2} & = (\L{f}{\L{x}{f (f x)}})\\
    \textbf{3} & = (\L{f}{\L{x}{f (f (f x))}})\\
%    \textbf{succ} & = \L{n}{\L{f}{\L{x}{f (n f x)}}}\\
%    \textbf{add} & = \L{m}{\L{n}{\L{f}{\L{x}{m f (n f x)}}}}\\
    \textbf{mult} & = \L{m}{\L{n}{\L{f}{\L{x}{m (n f) x}}}}
  \end{align*}

  \begin{solutionbox}{12cm}
  \begin{align*}
    \textbf{mult 3 2} &
     = (\L{m}{\L{n}{\L{f}{\L{x}{~m~(n f)~x}}}})~\textbf{3 2} & \\
    & \Rightarrow (\L{n}{\L{f}{\L{x}{~\textbf{3}~(n f)~x}}})~\textbf{2}\\
    & \Rightarrow \L{f}{\L{x}{~\textbf{3}~(\textbf{2}~f)~x}}\\
    & = \L{f}{\L{x}{~\textbf{3}~((\L{f}{\L{x}{f (f x)}})~f)~x}} & \textrm{expanded \textbf{2}}\\
    & = \L{f}{\L{x}{~\textbf{3}~(\underline{(\L{f}{\L{x}{f (f x)}})~f})~x}} & \textrm{$\beta$-reducing underlined term}\\
    & \Rightarrow \L{f}{\L{x}{~\textbf{3}~(\L{x}{f (f x)})~x}} & \\
    & = \L{f}{\L{x}{~(\L{f}{\L{x}{f (f (f x))}})~(\L{x}{f (f x)})~x}} & \textrm{expanded \textbf{3}}\\
    & = \L{f}{\L{x}{~\underline{(\L{f}{\L{x}{f (f (f x))}})~(\L{x}{f (f x)})}~x}} & \textrm{$\beta$-reducing underlined term}\\
    & \Rightarrow \L{f}{\L{x}{~(\L{x}{(\L{x}{f (f x)})~((\L{x}{f (f x)})~((\L{x}{f (f x)})~x))})~x}} & \\
    & = \L{f}{\L{x}{~(\L{x}{(\L{x}{f (f x)})~((\L{x}{f (f x)})~(\underline{(\L{x}{f (f x)})~x}))})~x}} & \textrm{$\beta$-reducing underlined term}\\
    & \Rightarrow \L{f}{\L{x}{~(\L{x}{(\L{x}{f (f x)})~((\L{x}{f (f x)})~(f (f x)))})~x}} & \\
    & = \L{f}{\L{x}{~(\L{x}{(\L{x}{f (f x)})~(\underline{(\L{x}{f (f x)})~(f (f x))})})~x}} & \textrm{$\beta$-reducing underlined term}\\
    & \Rightarrow \L{f}{\L{x}{~(\L{x}{(\L{x}{f (f x)})~(f (f (f (f x))))})~x}} & \\
    & = \L{f}{\L{x}{~(\L{x}{\underline{(\L{x}{f (f x)})~(f (f (f (f x))))}})~x}} & \textrm{$\beta$-reducing underlined term}\\
    & \Rightarrow \L{f}{\L{x}{~(\L{x}{(f (f (f (f (f (f x))))))})~x}} & \\
    & = \L{f}{\L{x}{~\underline{(\L{x}{(f (f (f (f (f (f x))))))})~x}}} & \textrm{$\beta$-reducing underlined term}\\
    & \Rightarrow \L{f}{\L{x}{(f (f (f (f (f (f x))))))}} & \\
    & = \textbf{6}
  \end{align*}
  \end{solutionbox}


\end{questions}
\end{document}
